type_soundness

swotarfe_andufotions/src/StlcProp.v
@@ -67,6 +67,8 @@ Inductive appears_free_in : id -> tm -> Prop :=
       appears_free_in x (tif c t e)
 .
 
+Hint Constructors appears_free_in.
+
 Definition closed (t : tm) :=
   forall x, ~ appears_free_in x t.
 
@@ -93,3 +95,77 @@ Proof.
 Qed.
 
 (* END typable_empty__closed. *)
+
+Lemma context_invariance : forall G G' t T,
+  G  |- t \in T ->
+  (forall x, appears_free_in x t -> G x = G' x) ->
+  G' |- t \in T.
+Proof with eauto.
+  intros G G' t T Hin Hst.
+  generalize dependent Hst. generalize dependent G'.
+  induction Hin; intros; eauto; econstructor...
+  - rewrite Hst in H...
+  - unfold pupdate in *.
+    apply IHHin; intros. unfold update. destruct (eq_id_dec i x0); subst...
+Qed.
+
+Lemma substitution_preserves_typing : forall G x U t v T,
+  pupdate G x U   |- t \in T ->
+  (fun _ => None) |- v \in U ->
+  G |- [x := v] t \in T.
+Proof with eauto.
+  unfold pupdate.
+  intros G x U t.
+  generalize dependent U. generalize dependent x. generalize dependent G.
+  induction t; simpl; intros; inversion H; subst...
+  - destruct (eq_id_dec i x0); subst.
+    + rewrite update_eq in H3. inversion H3; subst.
+      eapply context_invariance...
+      intros.
+      apply typable_empty__closed in H0. unfold closed in H0.
+      apply H0 in H1. contradiction.
+    + rewrite update_neq in H3...
+  - unfold pupdate in *.
+    destruct (eq_id_dec i x0); subst.
+    + eapply context_invariance...
+      intros. inversion H1; subst.
+      rewrite update_neq...
+    + econstructor. unfold pupdate.
+      eapply IHt...
+      eapply context_invariance...
+      intros.
+      rewrite update_permute...
+Qed.
+
+Theorem preservation : forall t t' T,
+  (fun _ => None) |- t \in T ->
+  t ==> t' ->
+  (fun _ => None) |- t' \in T.
+Proof with eauto.
+  remember (fun _ => (None : option ty)) as G.
+  intros t t' T Ht. generalize dependent t'.
+  induction Ht; intros; try solve by inversion.
+  - inversion H; subst...
+    + apply substitution_preserves_typing with T11...
+      * inversion Ht1...
+  - inversion H; subst...
+Qed.
+
+(* Exercise: 2 stars, optional (type_soundness) *)
+
+Definition stuck (t : tm) : Prop :=
+  (normal_form step) t /\ ~ value t.
+
+Corollary soundness : forall t t' T,
+  (fun _ => None) |- t \in T ->
+  t ==>* t' ->
+  ~(stuck t').
+Proof.
+  intros t t' T Hhas_type Hmulti. unfold stuck.
+  intros [Hnf Hnot_val]. unfold normal_form in Hnf.
+  induction Hmulti.
+  - apply progress in Hhas_type. destruct Hhas_type; contradiction.
+  - apply preservation with (t' := y0) in Hhas_type; eauto.
+Qed.
+
+(* END type_soundness. *)
